dimsum_examples/iris/unfinished_echo.v
@@ -1,0 +1,927 @@
+From iris.proofmode Require Import proofmode.
+From iris.bi.lib Require Import fixpoint.
+From dimsum.examples.iris Require Import asm rec2.
+Set Default Proof Using "Type".
+
+Local Open Scope Z_scope.
+
+Arguments subst_static _ !_ /.
+
+Definition echo_rec : fndef := {|
+  fd_args := [];
+  fd_static_vars := [];
+  fd_vars := [];
+  fd_body := LetE "c" (rec.Call (Val (ValFn "getc")) []) $
+             LetE "_" (rec.Call (Val (ValFn "putc")) [Var "c"]) $
+             LetE "c" (rec.Call (Val (ValFn "getc")) []) $
+             LetE "_" (rec.Call (Val (ValFn "putc")) [Var "c"]) $
+             Val (ValNum 0);
+  fd_static := I
+|}.
+
+Definition echo_prog : gmap string fndef :=
+  <["echo" := echo_rec]> $ ∅.
+
+(* Call with direct return *)
+Definition TCallRet {S} (f : string) (vs : list val) (h : heap_state) :
+  spec rec_event S (val * heap_state) :=
+  TVis (Outgoing, ERCall f vs h);;
+  e ← TExist _;
+  TVis (Incoming, e);;
+  if e is ERReturn v h' then
+    TRet (v, h')
+  else
+    TUb.
+
+Section TCallRet.
+
+  Context `{!dimsumGS Σ} `{!specGS} {S : Type}.
+
+  Lemma sim_src_TCallRet f vs h (k: _ → spec rec_event S void) Π Φ :
+    switch Π ({{κ σ POST,
+      ∃ f' vs' h1,
+      ⌜f' = f⌝ ∗ ⌜vs' = vs⌝ ∗ ⌜h1 = h⌝ ∗ ⌜κ = Some (Outgoing, ERCall f vs h)⌝ ∗
+    POST Src _ (spec_trans rec_event S) ({{σ' Π',
+      ⌜σ = σ'⌝ ∗  ∃ e,
+    switch Π' ({{κ σ POST,
+      ⌜κ = Some (Incoming, e)⌝ ∗
+    POST Src _ (spec_trans rec_event S) ({{ σ'' Π'',
+      ⌜σ = σ''⌝ ∗ ⌜Π = Π''⌝ ∗ (∀ v h', ⌜e = ERReturn v h'⌝ -∗ Φ (k (v, h'))) }})}})}})}}) -∗
+    SRC (Spec.bind (TCallRet f vs h) k) @ Π {{ Φ }}.
+  Proof.
+    iIntros "HC" => /=. rewrite /TCallRet bind_bind.
+    iApply sim_gen_TVis. iIntros (s) "Hs". iIntros "% % /=". iIntros "[% [% HΠ]]". subst.
+    iApply "HC" => /=. iSplit!.
+    iIntros (??) "[% [% HC]]" => /=. subst.
+    iApply (sim_gen_expr_intro _ tt with "[Hs] [-]"); simpl; [done..|]. rewrite bind_bind.
+    iApply (sim_src_TExist _). rewrite bind_bind.
+    iApply sim_gen_TVis. iIntros (s') "Hs". iIntros (??) "[% [% HΠ']]" => /=.
+    subst. iApply "HC" => /=. iSplit!.
+    iIntros (??) "[% [% HC]]". destruct!/=.
+    iApply "HΠ". iSplit!. iSplitL "Hs". 1: done.
+    destruct e. iApply sim_src_TUb.
+    rewrite bind_ret_l.
+    iApply sim_gen_expr_stop.
+    by iApply "HC".
+  Qed.
+
+End TCallRet.
+
+(* ********************************************************************************************** *)
+(* combined rec program that will return increasing numbers with each call *)
+(* ********************************************************************************************** *)
+Section sim_getc.
+  Context `{!dimsumGS Σ} `{!recGS Σ}.
+
+  Definition getc_spec : spec rec_event Z void :=
+    Spec.forever(
+    '(f, vs, h) ← TReceive (λ '(f, vs, h), (Incoming, ERCall f vs h));
+    TAssume (f = "getc");;
+    TAssume (vs = []);;
+    v ← TGet;
+    TPut (v + 1);;
+    TVis (Outgoing, ERReturn (ValNum v) h)).
+
+  Definition getc_spec_body : spec rec_event Z unit :=
+    '(f, vs, h) ← TReceive (λ '(f, vs, h), (Incoming, ERCall f vs h));
+    TAssume (f = "getc");;
+    TAssume (vs = []);;
+    v ← TGet;
+    TPut (v + 1);;
+    TVis (Outgoing, ERReturn (ValNum v) h).
+
+  Lemma mstate_var_agree {S : TypeState} `{!mstateG Σ} γ (σ1 σ2 : S) :
+    γ ⤳ σ1 -∗ γ ⤳ σ2 -∗ ⌜σ1 = σ2⌝.
+  Proof.
+    iIntros "H1 H2". iDestruct (ghost_var_agree with "[H1] [H2]") as %[=]; [done..|].
+    inv H0. by dimsum.core.axioms.simplify_K.
+  Qed.
+
+  Lemma sim_getc_spec `{!specGS} Π Φ :
+    switch Π ({{ κ σ1 POST,
+      ∃ f es h, ⌜κ = Some (Incoming, ERCall f es h)⌝ ∗
+    POST Tgt _ _ ({{ σ' Π',
+      ∃ v, ⌜f = "getc"⌝ ∗ ⌜es = []⌝ ∗ spec_state v ∗ ⌜σ' = σ1⌝ ∗
+    switch Π' (λ κ (σ : m_state (spec_trans rec_event Z)) POST,
+      ⌜κ = Some (Outgoing, ERReturn (ValNum v) h)⌝ ∗ spec_state (v + 1) ∗
+    POST Tgt _ _ ({{σ' Π'',
+      ⌜σ' = σ⌝ ∗ ⌜Π'' = Π⌝ ∗ TGT getc_spec @ Π {{ Φ }}
+    }}))}})}}) -∗
+    TGT getc_spec @ Π {{ Φ }}.
+  Proof.
+    iIntros "Hs".
+    rewrite {2}/getc_spec unfold_forever /TReceive bind_bind -/getc_spec bind_bind.
+    iApply (sim_tgt_TExist with "[-]"). iIntros ([[??]?]) "!>".
+    rewrite bind_bind. setoid_rewrite bind_ret_l.
+    iApply (sim_gen_TVis with "[-]").
+    iIntros (v') "Hγ' !>".
+    iIntros (??) "[% [% HΠ]]".
+    subst.
+    iApply "Hs" => /=. iSplit!. iIntros (??) => /=.
+    iDestruct 1 as (???) "[Hγ [% Hs']]". subst.
+    iApply (sim_gen_expr_intro _ tt with "[Hγ']"); simpl; [done..|]. rewrite bind_bind.
+    iApply (sim_tgt_TAssume with "[-]"); [done|]. iIntros "!>". rewrite bind_bind.
+    iApply (sim_tgt_TAssume with "[-]"); [done|]. iIntros "!>". rewrite bind_bind.
+    iApply (sim_gen_TGet with "[-]").
+    iSplit. 1: done.
+    iIntros "!>". rewrite bind_bind.
+    iApply (sim_gen_TPut with "[Hγ]"). 1: done.
+    iIntros "Hγ". iIntros "!>".
+    iApply (sim_gen_TVis with "[-]"). iIntros (v'') "Hγ'".
+    iDestruct (mstate_var_agree with "Hγ Hγ'") as "<-".
+    iIntros "!> /=".
+    iIntros (??) "[% [% HΠ']]" => /=. simplify_eq.
+    iApply "Hs'". iSplit!. iFrame.
+    iIntros (??) "[-> [-> HC]]".
+    iApply "HΠ" => /=. by iFrame.
+  Qed.
+
+  Definition getc_fn_spec (P : Z → iProp Σ) (es : list expr) (POST : (val → iProp Σ) → iProp Σ) : iProp Σ :=
+    ∃ v, P v ∗ ⌜es = []⌝ ∗ POST (λ ret, ⌜ret = v⌝ ∗ P (v + 1))%I.
+
+  (* I think this is the wrong level of abstraction *)
+  (* This is not a spec for getc, this is a spec of calling getc in the linked module *)
+  (* While the P is abstract, in the Proof itself, the P will capture whatever the PL is *)
+  Lemma sim_getc fns Π_l Π_r (PL : m_state (spec_trans rec_event Z) → iProp Σ) (σi : (m_state (spec_trans rec_event Z))) :
+    rec_fn_auth fns -∗
+    "getc" ↪ None -∗
+    PL σi -∗
+    ⌜σi.1 ≡ getc_spec⌝ -∗
+    ⌜σi.2 = 0⌝ -∗
+    □ switch_link_fixed Tgt Π_l (spec_trans _ Z) Π_r ({{σ_l POST,
+      ∃ h v σg, PL σg ∗
+    POST (ERCall "getc" [] h) σg ({{σ_r Π_r',
+    switch_link Tgt Π_r' ({{σ_r' POST,
+      ∃ h',
+    POST (ERReturn (ValNum v) h') _ σ_l ({{_ Π_l',
+      ⌜Π_l' = Π_l⌝ ∗ PL σ_r'
+    }})}})}})}}) -∗
+    |==> ∃ P, P 0 ∗ □ rec_fn_spec_hoare Tgt Π_l "getc" (getc_fn_spec P).
+  (* ⥥ₜ({{σ Π, ⌜σ = σg⌝ ∗ ⌜Π = Π_r⌝ ∗ TGT getc_spec @ Π {{Φg}}}}) ∗ *)
+  Proof.
+    iIntros "#? #? HPL %<-  #Hs".
+
+    iMod (mstate_var_alloc Z) as (γ) "Hγ".
+    iMod (mstate_var_split γ σi.2 with "[$]") as "[Hγ Hγ']".
+    pose (HS := SpecGS γ).
+
+    set P := (λ (v : Z), ∃ σ Φg, PL σ ∗ spec_state v ∗
+                           ⥥ₜ({{σ' Π, ⌜σ' = σ⌝ ∗ ⌜Π = Π_r⌝ ∗ TGT getc_spec @ Π {{Φg}}}}))%I.
+    iExists P.
+    iModIntro. iSplit.
+    - iExists _, (λ e, sim_post Tgt () Π_r e).
+      iFrame.
+      iIntros (??) "[-> [-> H]]" => /=.
+      iApply (sim_gen_expr_intro with "[Hγ]") => /= //.
+    - iIntros "!> %% [% [[% [% [HPL [Hγ Hg]]]] [-> HΦ]]]".
+      iApply (sim_tgt_rec_Call_external with "[$]").
+      iIntros (???) "#?Htoa Haa !>".
+      iIntros (? σr) "[-> [-> HΠr]]" => /=. subst.
+      iApply "Hs" => /=. iFrame. iSplit!.
+      iIntros (? Π'') "[-> [-> Hs']]" => /=.
+      iApply "Hg". iSplit!.
+      iApply sim_getc_spec.
+      iIntros (??) "[% [% [% [-> Hg]]]]" => /=.
+      iApply "Hs'" => /=. iSplit!.
+      iIntros (? Πs') "[% [% Hs']]". simplify_eq.
+      iApply "Hg". iFrame. iSplit!.
+      iIntros (??) "[-> [? Hg]]" => /=.
+      iApply "Hs'" => /=. iSplit!.
+      iIntros (? Πr') "[-> Hs']".
+      iApply sim_tgt_rec_Waiting_raw.
+      iSplit. { iIntros. iModIntro. iApply "Hs'". iSplit!. iIntros (??) "[% [% ?]]". simplify_eq. }
+      iIntros (???) "!>". iApply "Hs'" => /=. iSplit!. iIntros (??) "[% [% [% HQ]]]". simplify_eq.
+      iApply "HΠr". iSplit!. iFrame.
+      iApply "HΦ". iFrame. iSplit!.
+      iIntros (??) "[-> [-> ?]]" => /=.
+      iApply "Hg". by iSplit!.
+  Qed.
+
+End sim_getc.
+
+(* ********************************************************************************************** *)
+(* Prove ⟦echo⟧_rec ⊕ ⟦getc⟧_spec ⪯ ⟦echo_getc⟧_spec *)
+(* ********************************************************************************************** *)
+
+Section echo_getc.
+
+  Context `{!dimsumGS Σ} `{!recGS Σ}.
+
+  Definition echo_getc_spec_body : spec rec_event Z unit :=
+    v ← TGet;
+    TPut (v + 1);;
+    h ← TExist _;
+    '(_, h') ← TCallRet "putc" [(ValNum v)] h;
+    TAssume (h = h').
+
+  Definition echo_getc_spec : spec rec_event Z void :=
+    '(f, vs, h) ← TReceive (λ '(f, vs, h), (Incoming, ERCall f vs h));
+    TAssume (f = "echo");;
+    TAssume (vs = []);;
+    Spec.forever echo_getc_spec_body.
+
+  Let m_t := rec_link_trans {["echo"]} {["getc"]} rec_trans (spec_trans rec_event Z).
+
+  Lemma echo_getc_sim :
+    rec_state_interp (rec_init echo_prog) None -∗
+    (* TODO: Not exactly sure what the list is *)
+    (MLFRun None, [], rec_init echo_prog, (getc_spec, 0)) ⪯{m_t,
+      spec_trans rec_event Z} (echo_getc_spec, 0).
+  Proof.
+    iIntros "[#Hfns [Hh Ha]] /=".
+
+    (* REVIEW: Am I saying here that I have r/w over the modules, and when I step through one *)
+    (* I ensure I cannot change the other by splitting the var? *)
+    (* Entire Source Module *)
+    iMod (mstate_var_alloc (m_state (spec_trans rec_event Z))) as (γs) "Hγs".
+    (* Entire Target Module *)
+    iMod (mstate_var_alloc (m_state m_t)) as (γt) "Hγt".
+    (* Event *)
+    iMod (mstate_var_alloc (option rec_event)) as (γκ) "Hγκ".
+
+    (* Source's spec state *)
+    iMod (mstate_var_alloc Z) as (γs_s) "?".
+    iMod (mstate_var_split γs_s 0 with "[$]") as "[Hγs_s Hγs_s']".
+    pose (HSrcSpec := SpecGS γs_s).
+
+    iApply (sim_tgt_constP_intro γt γs γκ with "Hγt Hγs Hγκ [-]"). iIntros "Hγs".
+    (* NOTE: I am fixing here the state of the spec in the source *)
+    iApply (sim_tgt_link_None with "[-]"). iIntros "!>" (??????).
+    (* NOTE: Case splitting on the linking case, which can only be a call because of the empty list  *)
+    (* TODO: What is the empty list here, is it previous events? *)
+    destruct!/=. case_match; destruct!/=.
+
+    (* NOTE: Changing to source module *)
+    iApply (sim_tgt_constP_elim γt γs γκ with "[Hγs] [-]"); [done..|].
+    iIntros "Hγs Hγt Hγκ".
+    (* NOTE: Now, going into module local reasoning - Giving up one half of the state *)
+    iApply (sim_gen_expr_intro (Λ := spec_mod_lang (H := HSrcSpec) _ _ ) _ tt with "[Hγs_s] [-]"); [simpl; done..|].
+    iEval (unfold echo_getc_spec). rewrite /TReceive bind_bind.
+    iApply (sim_src_TExist (H := HSrcSpec) (_, _, _)). rewrite bind_bind .
+    setoid_rewrite bind_ret_l.
+    iApply (sim_gen_TVis (H := HSrcSpec)). iIntros "% Hγs_s %% [-> [-> _ ]]".
+
+    iApply (sim_src_constP_next with "[Hγt] [Hγκ] [Hγs] [%] [-]"); [done..|].
+    (* NOTE: I unify here *)
+    iDestruct (mstate_var_agree with "Hγs_s Hγs_s'") as "->".
+
+    iIntros "Hγs". iApply sim_gen_stop.
+    (* NOTE: I am here going right back into the src module, to get the function name from the assume *)
+    iApply (sim_tgt_constP_elim γt γs γκ with "[Hγs] [-]"); [done..|].
+    iIntros "Hγs Hγt Hγκ".
+
+    iApply (sim_gen_expr_intro (Λ := spec_mod_lang (H := HSrcSpec) _ _ ) _ tt with "[Hγs_s] [-]"); [simpl; done..|].
+    iApply (sim_src_TAssume (H := HSrcSpec)). iIntros (?).
+    iApply (sim_src_TAssume (H := HSrcSpec)). iIntros (?). simplify_eq.
+    iApply sim_gen_expr_None => /=. iIntros (? [] ?) "Hγs_s".
+
+    (* iDestruct (mstate_var_merge with "Hγs_s Hγs_s'") as "[<- Hγs_s]". *)
+    iIntros (??) "[-> [-> _]]".
+
+    (* NOTE: Changing into target *)
+    rewrite bool_decide_true; [|done].
+
+    (* NOTE: Maybe do induction here? *)
+
+    iDestruct (mstate_var_merge with "Hγs_s' Hγs_s") as "[% Hγs_s]".
+
+    iApply (sim_src_constP_next with "[Hγt] [Hγκ] [Hγs] [%] [-]"); [done..|].
+    iIntros "Hγs".
+    iApply (sim_tgt_link_recv_left with "[-]").
+    iApply (sim_tgt_rec_Waiting_raw _ []).
+    iSplit; [|by iIntros].
+    iIntros (???? Hin) "!> %". simplify_map_eq.
+
+    (* TODO: Maybe it's better not to keep the spec state around *)
+    (* Target's spec module (Right linking case - getc) *)
+    iMod (mstate_var_alloc (m_state (spec_trans rec_event Z))) as (γt_r) "Hγt_r".
+
+    (* Target's right spec state*)
+    iMod (mstate_var_alloc Z) as (γt_r_s) "Hγt_r_s".
+    pose (HTgtSpec := SpecGS γt_r_s).
+
+    (* TODO: "queue" for linking?  *)
+    iMod (mstate_var_alloc (list seq_product_case)) as (γt_q) "Hγt_q".
+
+    (* Linking event to pass around *)
+    iMod (mstate_var_alloc (option rec_ev)) as (γt_oe) "Hγt_oe".
+
+    iApply (sim_tgt_link_left_const_run γt_q γt_r γt_oe with "[$] [$] [$] [-]").
+    iIntros "Hγt_q Hγt_r Hγt_oe".
+
+    iMod (rec_mapsto_alloc_big (h_heap h) with "Hh") as "[Hh _]". { apply map_disjoint_empty_r. }
+
+    set (Πl := tgt_link_left_constP _ _ _ _ _).
+
+    iApply (sim_gen_expr_intro _ [] with "[Hh Ha]"). { done. }
+    { rewrite /= /rec_state_interp dom_empty_L right_id_L /=. iFrame "#∗". by iApply rec_alloc_fake. }
+
+    iApply (sim_gen_expr_bind _ [ReturnExtCtx _] with "[-]") => /=.
+
+    (* TODO: HERE INDUCTION *)
+
+    (* TODO: Awkward to do this here *)
+    iApply sim_gen_expr_ctx. iIntros "#?".
+
+    iMod (mstate_var_alloc (m_state rec_trans)) as (γt_l) "Hγt_l".
+
+    set P := (λ (σ : spec rec_event Z void * Z),
+                γt_l ⤳@{(m_state rec_trans)} - ∗ γt_r ⤳ σ ∗
+                γt_oe ⤳ @None rec_ev ∗ γt_q ⤳ [None : seq_product_case])%I.
+    iDestruct (sim_getc _ Πl _ P (getc_spec, 0) with "[$] [] [$] [//] [//]") as "H".
+    { by iApply (rec_fn_intro with "[$]"). }
+    iMod ("H" with "[]") as "[% [HP #Hgetc]]".
+
+    { iIntros "!> %% [% [% [% [[Hγt_l [Hγt_r [Hγt_oe Hγt_q]]] [% HC]]]]]" => /=. subst.
+      iIntros (???) "Hγt_q' Hγt_r' Hγt_oe'".
+
+      iDestruct (mstate_var_merge with "Hγt_r Hγt_r'") as "[<- Hγt_r]".
+      iDestruct (mstate_var_merge with "Hγt_oe Hγt_oe'") as "[<- Hγt_oe]".
+      iDestruct (mstate_var_merge with "Hγt_q Hγt_q'") as "[<- Hγt_q]".
+
+      iIntros (??????).
+      destruct!/=. rewrite bool_decide_false //. rewrite bool_decide_true //.
+
+      (* iApply (sim_tgt_link_left_const_recv γt_q γt_r γt_oe with "[$] [Hγt_r] [$] [-]"). 1: done. *)
+      iApply (sim_tgt_link_right_const_recv γt_q γt_l γt_oe with "[$] [Hγt_l] [$] [-]"). 1: done.
+      iIntros "Hγt_q Hγt_l Hγt_oe".
+      iApply "HC". iSplit!.
+      iIntros (??) "[% [-> HC]]"=> /=.
+      iIntros (???) "Hγt_q' Hγt_l' Hγt_oe'".
+
+      iDestruct (mstate_var_merge with "Hγt_l Hγt_l'") as "[<- Hγt_l]".
+      iDestruct (mstate_var_merge with "Hγt_oe Hγt_oe'") as "[<- Hγt_oe]".
+      iDestruct (mstate_var_merge with "Hγt_q Hγt_q'") as "[<- Hγt_q]".
+
+      iIntros (?). simplify_eq.
+
+      iApply (sim_tgt_link_right_const_run γt_q γt_l γt_oe with "[$] [Hγt_l] [$] [-]"). 1: done.
+      iIntros "Hγt_q Hγt_l Hγt_oe".
+      iApply "HC" => /=. iSplit!.
+      iIntros (??) "[% [-> HC]]". simpl.
+      iIntros (???) "Hγt_q' Hγt_l' Hγt_oe'".
+
+      iDestruct (mstate_var_merge with "Hγt_l Hγt_l'") as "[<- Hγt_l]".
+      iDestruct (mstate_var_merge with "Hγt_oe Hγt_oe'") as "[<- Hγt_oe]".
+      iDestruct (mstate_var_merge with "Hγt_q Hγt_q'") as "[<- Hγt_q]".
+
+      iIntros (??????).
+      destruct!/=.
+
+      iApply (sim_tgt_link_left_const_recv γt_q γt_r γt_oe with "[$] [Hγt_r] [$] [-]"). 1: done.
+      iIntros "Hγt_q Hγt_r Hγt_oe".
+      iApply "HC". iSplit!.
+      iIntros (??) "[% [-> HC]]" => /=.
+
+      iIntros (?) "%% Hγt_q' Hγt_r' Hγt_oe'".
+
+      iDestruct (mstate_var_merge with "Hγt_oe Hγt_oe'") as "[<- Hγt_oe]".
+      iDestruct (mstate_var_merge with "Hγt_q Hγt_q'") as "[<- Hγt_q]".
+      iDestruct (mstate_var_merge with "Hγt_r Hγt_r'") as "[<- Hγt_r]".
+
+      iIntros (?). simplify_eq.
+      iApply (sim_tgt_link_left_const_run γt_q γt_r γt_oe with "[$] [Hγt_r] [$] [-]"). 1: done.
+      iIntros "Hγt_q Hγt_r Hγt_oe".
+      iApply "HC". iSplit!. iFrame.
+    }
+
+    iAssert (∀ Φ σ, ⌜σ.1 ≡ Spec.forever echo_getc_spec_body⌝ -∗ γs ⤳ σ -∗
+                    γs_s ⤳ - -∗ γt_r_s ⤳ - -∗
+                    γt_oe ⤳ None -∗ γt_r ⤳ (getc_spec, σ.2) -∗ γt_q ⤳ [None] -∗
+                    TGT Call (Val (ValFn "echo")) [] @ Π {{ Φ }})%I as "H".
+    {
+      iApply (ord_loeb with "[$] []").
+      iIntros "!>". iIntros "#IH % % % Hγs Hγs_s Hγt_r_s Hγt_oe Hγt_r Hγt_q".
+
+      iMod (mstate_var_split γt_r_s σ0.2 with "[$]") as "[Hγt_r_s Hγt_r_s']".
+
+      rewrite /echo_prog in Hin. simplify_map_eq.
+      (* NOTE: Here, first attempt of proving it with no intermediate lemmas *)
+      iApply (sim_tgt_rec_Call_internal); [ | by iApply (rec_fn_intro with "[$]") |]. { done. }
+      iModIntro => /=.
+      iApply (sim_tgt_rec_AllocA); [done|].
+      iIntros "% _ !>" => /=.
+      iApply (sim_gen_expr_bind _ [LetECtx _ _] with "[-]") => /=.
+
+      iDestruct (sim_getc with "[$] [] [] [] []") as "H". [by iApply (rec_fn_intro with "[$]")|].
+
+      iApply sim_tgt_rec_Call_external;[by iApply (rec_fn_intro with "[$]")|].
+      iIntros (???) "_ Hma Haa !>".
+
+      (* NOTE: Here I am throwing out way back in *)
+      iIntros (??) "[% [% HΠ]]" => /=. subst.
+      iIntros (???) "Hγt_q' Hγt_r' Hγt_oe'".
+
+      iDestruct (mstate_var_merge with "Hγt_r Hγt_r'") as "[<- Hγt_r]".
+      iDestruct (mstate_var_merge with "Hγt_oe Hγt_oe'") as "[<- Hγt_oe]".
+      iDestruct (mstate_var_merge with "Hγt_q Hγt_q'") as "[<- Hγt_q]".
+
+      iIntros (??????).
+      destruct!/=. rewrite bool_decide_false //. rewrite bool_decide_true //.
+      iApply (sim_tgt_link_recv_right with "[-]").
+      iApply (sim_gen_expr_intro _ tt with "[Hγt_r_s]"); simpl; [done..|].
+      rewrite {2}/getc_spec unfold_forever /TReceive bind_bind bind_bind -/getc_spec.
+      iApply (sim_tgt_TExist with "[-]"). iIntros ([[??]?]) "!>".
+      rewrite bind_bind. setoid_rewrite bind_ret_l.
+      iApply (sim_gen_TVis with "[-]").
+      (* NOTE: Throwing out more stuff *)
+      iIntros (v) "Hγt_r_s !>". iIntros (??) "[% [% _]]". subst.
+      iIntros (?). simplify_eq.
+
+      iDestruct (mstate_var_agree with "Hγt_r_s Hγt_r_s'") as "->".
+
+      iApply (sim_tgt_link_run_right with "[-]").
+      iApply (sim_gen_expr_intro _ tt with "[Hγt_r_s]"); simpl; [done..|]. rewrite bind_bind.
+      iApply sim_tgt_TAssume; [done|]. iModIntro. rewrite bind_bind.
+      iApply sim_tgt_TAssume; [done|]. iModIntro. rewrite bind_bind.
+      iApply (sim_gen_TGet with "[-]").
+      iSplit. 1: done.
+      iIntros "!>". rewrite bind_bind.
+      iApply (sim_gen_TPut with "[Hγt_r_s']"). 1: done.
+      iIntros "Hγt_r_s' !>" => /=.
+      iApply (sim_gen_TVis with "[-]"). iIntros (?) "Hγt_r_s !>".
+
+      iDestruct (mstate_var_agree with "Hγt_r_s Hγt_r_s'") as "->".
+
+      (* NOTE: Throwing out stuff again *)
+      iIntros (??) "[% [% _]]" => /=. subst.
+      iIntros (??????). destruct!/=.
+
+      iApply (sim_tgt_link_left_const_recv γt_q γt_r γt_oe with "[$] [Hγt_r] [$] [-]"). 1: done.
+      iIntros "Hγt_q Hγt_r Hγt_oe".
+      iApply sim_tgt_rec_Waiting_all_raw. iIntros (?) "!> %%% Hγt_q' Hγt_r' Hγt_oe'".
+
+      iDestruct (mstate_var_merge with "Hγt_oe Hγt_oe'") as "[<- Hγt_oe]".
+      iDestruct (mstate_var_merge with "Hγt_q Hγt_q'") as "[<- Hγt_q]".
+      iDestruct (mstate_var_merge with "Hγt_r Hγt_r'") as "[<- Hγt_r]".
+      iIntros (?). simplify_eq.
+
+      iApply (sim_tgt_link_left_const_run γt_q γt_r γt_oe with "[$] [$] [$] [-]").
+      iIntros "Hγt_q Hγt_r Hγt_oe".
+      (* NOTE - finally going back in *)
+      iApply "HΠ". iSplit!. iFrame.
+
+      iApply sim_tgt_rec_LetE. iModIntro => /=.
+      iApply (sim_gen_expr_bind _ [LetECtx _ _] with "[-]") => /=.
+
+      iApply sim_tgt_rec_Call_external;[by iApply (rec_fn_intro with "[$]")|].
+      iIntros (???) "_ ? ? !> %% [% [% HΠ]] %%% Hγt_q' Hγt_r' Hγt_oe'" => /=. subst.
+
+      iDestruct (mstate_var_merge with "Hγt_oe Hγt_oe'") as "[<- Hγt_oe]".
+      iDestruct (mstate_var_merge with "Hγt_q Hγt_q'") as "[<- Hγt_q]".
+      iDestruct (mstate_var_merge with "Hγt_r Hγt_r'") as "[<- Hγt_r]".
+
+      iIntros (??????).
+      destruct!/=. rewrite bool_decide_false //.
+      iIntros (?) "Hγs' Hγκ Hγt".
+
+      iDestruct (mstate_var_merge with "Hγs Hγs'") as "[<- Hγs]".
+
+      iMod (mstate_var_split γs_s σ0.2 with "[$]") as "[Hγs_s Hγs_s']".
+
+      iApply (sim_gen_expr_intro (Λ := spec_mod_lang (H := HSrcSpec) _ _ ) _ tt with "[Hγs_s] [-]"); simpl; [done.. |].
+
+      rewrite {2}unfold_forever /echo_getc_spec_body bind_bind -/echo_getc_spec_body.
+      iApply (sim_gen_TGet (H := HSrcSpec) with "[-]"). iSplit. 1: done. rewrite bind_bind.
+      iApply (sim_gen_TPut (H := HSrcSpec) with "[$]"). iIntros "Hγs_s". rewrite bind_bind.
+      iApply (sim_src_TExist (H := HSrcSpec)). rewrite !bind_bind.
+      iApply (sim_gen_TVis (H := HSrcSpec) with "[-]"). iIntros (?) "Hγs_s'".
+      iDestruct (mstate_var_agree with "Hγs_s Hγs_s'") as "<-".
+      iIntros (??) "[% [% _]]" => /=. simplify_eq.
+      iApply (sim_src_constP_elim with "[Hγt] [Hγκ //] [-]"). 1: done.
+      iIntros "Hγt Hγκ". iSplit!.
+
+      iApply (@sim_tgt_constP_intro _ _ _ m_t (spec_trans rec_event Z) γt γs γκ with "Hγt Hγs Hγκ").
+      iIntros "Hγs".
+
+      iApply (sim_tgt_link_None with "[-]"). iIntros "!>" (??????).
+
+      destruct!/=. case_match; destruct!/=.
+      { (* Incoming Call *)
+        iApply (sim_tgt_constP_elim γt γs γκ with "[Hγs] [-]"); [done..|].
+        iIntros "Hγs Hγt Hγκ".
+        iApply (sim_gen_expr_intro (Λ := spec_mod_lang (H := HSrcSpec) _ _ ) _ tt with "[Hγs_s] [-]"); [simpl; done..|].
+        rewrite bind_bind.
+        iApply (sim_src_TExist (H := HSrcSpec)).
+        rewrite bind_bind.
+        iApply (sim_gen_TVis (H := HSrcSpec) with "[-]"). iIntros (?) "Hγs_s".
+        iIntros (??) "[% [% ?]]"=> /=.
+        iApply (sim_src_constP_elim γt γκ with "[Hγt] [Hγκ] [-]"); [done..|].
+        iIntros "Hγt Hγκ". iSplit!.
+
+        (* TODO : This is quite annoying *)
+        iApply (@sim_tgt_constP_intro _ _ _ m_t (spec_trans rec_event Z) γt γs γκ with "Hγt Hγs Hγκ [-]"). iIntros "Hγs".
+        iApply (sim_gen_stop).
+
+        iApply (sim_tgt_constP_elim γt γs γκ with "[Hγs] [-]"); [done..|]. iIntros "Hγs Hγt Hγκ".
+        subst.
+        iApply (sim_gen_expr_intro (Λ := spec_mod_lang (H := HSrcSpec) _ _ ) _ tt with "[Hγs_s] [-]"); [simpl; done..|].
+        iApply (sim_src_TUb (H := HSrcSpec)).
+      }
+
+      iApply (sim_tgt_constP_elim γt γs γκ with "[Hγs] [-]"); [done..|].
+      iIntros "Hγs Hγt Hγκ".
+      iApply (sim_gen_expr_intro (Λ := spec_mod_lang (H := HSrcSpec) _ _ ) _ tt with "[Hγs_s] [-]"); [simpl; done..|].
+      rewrite bind_bind.
+      iApply (sim_src_TExist (H := HSrcSpec)).
+      rewrite bind_bind.
+      iApply (sim_gen_TVis (H := HSrcSpec) with "[-]"). iIntros (?) "Hγs_s".
+      iIntros (??) "[% [% ?]]"=> /=.
+      iApply (sim_src_constP_elim γt γκ with "[Hγt] [Hγκ] [-]"); [done..|].
+      iIntros "Hγt Hγκ". iSplit!.
+
+      (* TODO : This is quite annoying *)
+
+      iApply (@sim_tgt_constP_intro _ _ _ m_t (spec_trans rec_event Z) γt γs γκ with "Hγt Hγs Hγκ [-]"). iIntros "Hγs".
+      iApply (sim_gen_stop).
+
+      iApply (sim_tgt_constP_elim γt γs γκ with "[Hγs] [-]"); [done..|]. iIntros "Hγs Hγt Hγκ".
+      subst.
+      iApply (sim_gen_expr_intro (Λ := spec_mod_lang (H := HSrcSpec) _ _ ) _ tt with "[Hγs_s] [-]"); [simpl; done..|].
+      setoid_rewrite bind_ret_l.
+      iApply (sim_src_TAssume (H := HSrcSpec)). iIntros "->".
+      iApply (sim_gen_expr_stop). iIntros (?) "/= % Hγs_s".
+      iApply (sim_gen_stop).
+
+
+      iApply (sim_src_constP_elim γt γκ with "[Hγt] [Hγκ] [-]"); [done..|].
+      iIntros "Hγt Hγκ". iSplit!.
+
+      iApply (@sim_tgt_constP_intro _ _ _ m_t (spec_trans rec_event Z) γt γs γκ with "Hγt Hγs Hγκ [-]"). iIntros "Hγs".
+      iApply (sim_tgt_link_left_const_recv γt_q γt_r γt_oe with "Hγt_q [Hγt_r] [Hγt_oe] [-]"); [done..|].
+      iIntros "Hγt_q Hγt_r Hγt_oe".
+      iApply sim_tgt_rec_Waiting_all_raw. iIntros (?) "!> %%% Hγt_q' Hγt_r' Hγt_oe'".
+
+      iDestruct (mstate_var_merge with "Hγt_oe Hγt_oe'") as "[<- Hγt_oe]".
+      iDestruct (mstate_var_merge with "Hγt_q Hγt_q'") as "[<- Hγt_q]".
+      iDestruct (mstate_var_merge with "Hγt_r Hγt_r'") as "[<- Hγt_r]".
+      iDestruct (mstate_var_merge with "Hγt_r_s Hγt_r_s'") as "[_ Hγt_r_s]".
+      iDestruct (mstate_var_merge with "Hγs_s Hγs_s'") as "[<- Hγs_s]".
+      iIntros (?). simplify_eq.
+
+      iApply (sim_tgt_link_left_const_run γt_q γt_r γt_oe with "Hγt_q [Hγt_r] [Hγt_oe] [-]"); [done..|].
+      iIntros "Hγt_q Hγt_r Hγt_oe".
+      iApply "HΠ" => /=. iSplit!. iFrame.
+      iApply sim_tgt_rec_LetE. iModIntro => /=.
+
+      iApply ("IH" with "[//] [$] [$] [$] [$] [$] [$]").
+    }
+    rewrite H0.
+    iApply ("H" with "[//] [$] [$] [$] [$] [$] [$]").
+  Qed.
+
+End echo_getc.
+
+(* Section echo_getc. *)
+
+(*   Context `{!dimsumGS Σ} `{!recGS Σ}. *)
+
+(*   Definition echo_getc_spec_body : spec rec_event Z unit := *)
+(*     v ← TGet; *)
+(*     TPut (v + 1);; *)
+(*     h ← TExist _; *)
+(*     '(_, h') ← TCallRet "putc" [(ValNum v)] h; *)
+(*     TAssume (h = h'). *)
+
+(*   Definition echo_getc_spec : spec rec_event Z void := *)
+(*     '(f, vs, h) ← TReceive (λ '(f, vs, h), (Incoming, ERCall f vs h)); *)
+(*     TAssume (f = "echo");; *)
+(*     TAssume (vs = []);; *)
+(*     echo_getc_spec_body;; *)
+(*     echo_getc_spec_body;; *)
+(*     h' ← TExist _; *)
+(*     TVis (Outgoing, ERReturn (ValNum 0) h');; *)
+(*     TUb. *)
+
+(*   Definition echo_left_linkP γ_oe γ_q γ_r : Z → iProp Σ := *)
+(*     (λ v, γ_oe ⤳ @None rec_ev ∗ γ_q ⤳ [None : seq_product_case] ∗ γ_r ⤳ (getc_spec, v))%I. *)
+
+(*   (* Here I will take two things, one is the state of the tgt and one of the src *) *)
+(*   Definition putc_echo_fn_spec (P : Z → (spec rec_event Z void) → iProp Σ) (Q : Z → iProp Σ) (es : list expr) (POST : (val → iProp Σ) → iProp Σ) : iProp Σ := *)
+(*     ∃ v k v', P v (Spec.bind echo_getc_spec_body (fun _ => k)) ∗ Q v' ∗ ⌜es = [Val v]⌝ ∗ *)
+(*            POST (λ _, Q v' ∗ P (v + 1)%Z k)%I. *)
+
+(*   Lemma sim_echo_body Π_t Π_s (P : Z → (spec rec_event Z void) → iProp Σ) (Q : Z → iProp Σ) : *)
+(*     "putc" ↪ None -∗ *)
+(*     switch_external_fixed Π_t (spec_trans _ Z) Π_s ({{κ0 σ_t POST0, *)
+(*       ∃ vs h v k (vq : Z) p, P v p ∗ Q vq ∗ ⌜p ≡ Spec.bind echo_getc_spec_body (fun _ => k)⌝ ∗ *)
+(*       ⌜κ0 = Some (Outgoing, ERCall "putc" vs h)⌝ ∗ *)
+(*     POST0 (p, v) ({{σ_s1' Π_s', *)
+(*       ∃ e : rec_ev, ⌜Π_s' = Π_s⌝ ∗ *)
+(*     switch Π_s' ({{ κ3 σ_s2 POST2, *)
+(*       ⌜κ3 = Some (Incoming, e)⌝ ∗ *)
+(*     POST2 Src _ (spec_trans _ Z) ({{ σ_s2' Π_s'', *)
+(*       ⌜Π_s'' = Π_s'⌝ ∗ ⌜σ_s2 = σ_s2'⌝ ∗ *)
+(*     switch Π_s ({{ κ4 σ_s3 POST3, *)
+(*       ∃ v' h', ⌜e = ERReturn v' h'⌝ ∗ ⌜κ4 = None⌝ ∗ ⌜σ_s3.1 ≡ k⌝ ∗ ⌜σ_s3.2 = (v + 1)%Z⌝ ∗ *)
+(*     POST3 Tgt _ _ ({{ σ_t1 Π_t', *)
+(*       ⌜σ_t1 = σ_t⌝ ∗ ⌜Π_t' = Π_t⌝ ∗ *)
+(*     switch Π_t ({{ κ5 σ_t2 POST4, *)
+(*       ∃ e' : rec_ev, ⌜κ5 = Some (Incoming, e')⌝ ∗ *)
+(*     POST4 Tgt rec_event rec_trans ({{ σ_t3 Π_t', *)
+(*       ⌜σ_t3 = σ_t2⌝ ∗ ⌜e = e'⌝ ∗ ⌜Π_t = Π_t'⌝ ∗ P (v + 1) k ∗ Q vq *)
+(*       }})}})}})}})}})}})}})}}) -∗ *)
+(*     rec_fn_spec_hoare Tgt Π_t "putc" (putc_echo_fn_spec P Q). *)
+(*   Proof. *)
+(*     iIntros "#? Hs %% [% [% [% [? [? [-> HΦ]]]]]]". *)
+
+(*     iApply (sim_tgt_rec_Call_external with "[$]"). *)
+(*     iIntros (???) "#? ? ? !> %% [-> [-> HΠ]]" => /=. *)
+(*     iApply "Hs" => /=. iFrame. iSplit!. 1: done. *)
+(*     iIntros (? Πs) "[-> [-> Hs']]" => /=. *)
+
+(*     iMod (mstate_var_alloc Z) as (γs_s) "?". *)
+(*     iMod (mstate_var_split γs_s v with "[$]") as "[Hγs_s Hγs_s']". *)
+(*     pose (HSrcSpec := SpecGS γs_s). *)
+
+(*     iApply (sim_gen_expr_intro (Λ := spec_mod_lang (H := HSrcSpec) _ _ ) _ tt with "[Hγs_s] [-]"); [simpl; done..|]. rewrite bind_bind. *)
+(*     iApply (sim_gen_TGet (H := HSrcSpec) with "[-]"). iSplit. 1: done. rewrite bind_bind. *)
+(*     iApply (sim_gen_TPut (H := HSrcSpec) with "[$]"). iIntros "Hγs_s". rewrite bind_bind. *)
+(*     iApply (sim_src_TExist (H := HSrcSpec)). rewrite bind_bind. *)
+
+(*     iApply sim_src_TCallRet. *)
+
+(*     iIntros (??) "[% [% [% [% [% [% [% Hσ]]]]]]]" => /=. simplify_eq. *)
+(*     iApply "Hs'". iSplit!. *)
+(*     iIntros (??) "[% [% [% Hs']]]" => /=. subst. *)
+(*     iApply "Hσ". iSplit!. iIntros (??) "[% Hσ0]". *)
+(*     iApply "Hs'". iSplit!. iIntros (??) "[% [% Hs']]". subst. *)
+(*     iApply "Hσ0". iSplit!. iIntros (??) "% % /= % Hγs_s'". subst. *)
+(*     iApply (sim_gen_expr_intro (Λ := spec_mod_lang (H := HSrcSpec) _ _ ) _ tt with "[Hγs_s'] [-]"); [simpl; done..|]. *)
+(*     iApply sim_src_TAssume. iIntros "->". iApply sim_gen_expr_stop. *)
+(*     iIntros (?) "/= % Hγs_s'". iApply sim_gen_stop. *)
+(*     iApply "Hs'" => /=. *)
+(*     iDestruct (mstate_var_agree with "Hγs_s Hγs_s'") as "<-". *)
+(*     iSplit!. *)
+(*     iIntros (??) "[-> [-> Hs']]". *)
+(*     iApply sim_tgt_rec_Waiting_all_raw. iIntros (?) "!>". *)
+(*     iApply "Hs'". iSplit!. iIntros (??) "[% [% [% [? ?]]]]" => /=. subst. *)
+(*     iApply "HΠ" => /=. iSplit!. iFrame. iApply "HΦ". iFrame. *)
+(*   Qed. *)
+
+(*   Lemma sim_echo Π (P : Z → iProp Σ) (Q : Z → (spec rec_event Z void) → iProp Σ) : *)
+(*     "echo" ↪ Some echo_rec -∗ *)
+(*     □ rec_fn_spec_hoare Tgt Π "getc" (getc_fn_spec P) -∗ *)
+(*     □ rec_fn_spec_hoare Tgt Π "putc" (putc_echo_fn_spec Q P) -∗ *)
+(*     rec_fn_spec_hoare Tgt Π "echo" (λ es POST, ∃ v k, ⌜es = []⌝ ∗ *)
+(*       P v ∗ Q v (Spec.bind echo_getc_spec_body (fun _ => (Spec.bind echo_getc_spec_body (fun _ => k)))) ∗ *)
+(*       POST (λ ret, P (v + 2) ∗ Q (v + 2) k ∗ ⌜ret = 0⌝)). *)
+(*   Proof. *)
+(*     iIntros "#? #Hgetc #Hputc". *)
+(*     iIntros (es Φ) => /=. iDestruct 1 as (v k ->) "[HP [HQ HΦ]]". *)
+(*     iApply sim_tgt_rec_Call_internal. 2: { done. } { done. } *)
+(*     iModIntro => /=. *)
+(*     iApply sim_tgt_rec_AllocA; [by econs|] => /=. iIntros (?) "Hoof !>". *)
+(*     iApply (sim_gen_expr_bind _ [LetECtx _ _] with "[-]") => /=. *)
+(*     (* getc 1 *) *)
+(*     iApply "Hgetc". iFrame. iSplit!. iIntros (?) "[-> ?]". *)
+(*     iApply sim_tgt_rec_LetE. iIntros "!>" => /=. *)
+(*     iApply (sim_gen_expr_bind _ [LetECtx _ _] with "[-]") => /=. *)
+(*     (* putc 1 *) *)
+(*     iApply "Hputc". iFrame. iSplit!. iIntros (?) "[? ?]". *)
+(*     iApply sim_tgt_rec_LetE. iIntros "!>" => /=. *)
+(*     iApply (sim_gen_expr_bind _ [LetECtx _ _] with "[-]") => /=. *)
+(*     (* getc 2 *) *)
+(*     iApply "Hgetc". iFrame. iSplit!. iIntros (?) "[-> ?]". *)
+(*     iApply sim_tgt_rec_LetE. iIntros "!>" => /=. *)
+(*     iApply (sim_gen_expr_bind _ [LetECtx _ _] with "[-]") => /=. *)
+(*     (* putc 2 *) *)
+(*     iApply "Hputc". iFrame. iSplit!. iIntros (?) "[? ?]". *)
+(*     iApply sim_tgt_rec_LetE. iIntros "!>" => /=. *)
+
+(*     iApply sim_gen_expr_stop. iSplit!. *)
+(*     iSplitL "Hoof". *)
+(*     { destruct ls; [by iApply big_sepL2_nil |done]. } *)
+(*     replace (v + 1 + 1) with (v + 2) by lia. *)
+(*     iApply "HΦ". by iFrame. *)
+(*   Qed. *)
+
+
+(*   Definition echo_left_external γs : Z → (spec rec_event Z void) → iProp Σ := *)
+(*     (λ v k, ∃ σ, γs ⤳ σ ∗ ⌜σ.1 ≡ k⌝ ∗ ⌜σ.2 = v⌝)%I. *)
+
+(*   Lemma sim_echo_full Π_t γs γ_oe γ_q γ_r (k : spec rec_event Z void) (v : Z) (σs : m_state (spec_trans rec_event Z)): *)
+(*     "echo" ↪ Some echo_rec -∗ *)
+(*     "getc" ↪ None -∗ *)
+(*     "putc" ↪ None -∗ *)
+(*     γs ⤳ σs -∗ *)
+(*     γ_oe ⤳ @None rec_ev -∗ *)
+(*     γ_q ⤳ [(None : seq_product_case)] -∗ *)
+(*     γ_r ⤳ (getc_spec, v) -∗ *)
+(*     ⌜σs.1 ≡ Spec.bind echo_getc_spec_body (fun _ => (Spec.bind echo_getc_spec_body (fun _ => k)))⌝ -∗ *)
+(*     ⌜σs.2 = v⌝ -∗ *)
+(*     □ rec_fn_spec_hoare Tgt Π_t "getc" (getc_fn_spec (echo_left_linkP γ_oe γ_q γ_r)) -∗ *)
+(*     □ rec_fn_spec_hoare Tgt Π_t "putc" (putc_echo_fn_spec (echo_left_external γs) (echo_left_linkP γ_oe γ_q γ_r)) -∗ *)
+(*     rec_fn_spec_hoare Tgt Π_t "echo" ({{ es POST_e, ⌜es = []⌝ ∗ *)
+(*       POST_e (λ v, ∃ (σs r: m_state (spec_trans rec_event Z)), *)
+(*                 ⌜v = 0⌝ ∗ γs ⤳ σs ∗ ⌜σs.1 ≡ k⌝ ∗ γ_oe ⤳ @None rec_ev ∗ γ_q ⤳ [(None : seq_product_case)] ∗ *)
+(*                 γ_r ⤳ r) *)
+(*     }}). *)
+(*   Proof. *)
+(*     iIntros "#?#?#? Hγs Hγ_oe Hγ_q Hγ_r %% #Hgetc #Hputc %% [-> HΦ]" => /=. *)
+(*     iApply (sim_echo with "[//] [$] [$]"). *)
+(*     iFrame. iSplit!. 1: { done. } *)
+(*     iIntros (?) "[? [[% [? [% %]]] %]]". *)
+(*     iApply "HΦ". *)
+(*     iSplit!. by iFrame. *)
+(*   Qed. *)
+
+(*   Let m_t := rec_link_trans {["echo"]} {["getc"]} rec_trans (spec_trans rec_event Z). *)
+
+(*   Lemma echo_getc_sim : *)
+(*     rec_state_interp (rec_init echo_prog) None -∗ *)
+(*     (MLFRun None, [], rec_init echo_prog, (getc_spec, 0)) ⪯{m_t, *)
+(*       spec_trans rec_event Z} (echo_getc_spec, 0). *)
+(*   Proof. *)
+(*     iIntros "[#Hfns [Hh Ha]] /=". *)
+
+(*     iMod (mstate_var_alloc (m_state (spec_trans rec_event Z))) as (γs) "Hγs". *)
+(*     (* Entire Target Module *) *)
+(*     iMod (mstate_var_alloc (m_state m_t)) as (γt) "Hγt". *)
+(*     (* Event *) *)
+(*     iMod (mstate_var_alloc (option rec_event)) as (γκ) "Hγκ". *)
+
+(*     (* Source's spec state *) *)
+(*     iMod (mstate_var_alloc Z) as (γs_s) "?". *)
+(*     iMod (mstate_var_split γs_s 0 with "[$]") as "[Hγs_s Hγs_s']". *)
+(*     pose (HSrcSpec := SpecGS γs_s). *)
+
+(*     iApply (sim_tgt_constP_intro γt γs γκ with "Hγt Hγs Hγκ [-]"). iIntros "Hγs". *)
+(*     iApply (sim_tgt_link_None with "[-]"). iIntros "!>" (??????). *)
+(*     destruct!/=. case_match; destruct!/=. *)
+
+(*     iApply (sim_tgt_constP_elim γt γs γκ with "[Hγs] [-]"); [done..|]. *)
+(*     iIntros "Hγs Hγt Hγκ". *)
+(*     iApply (sim_gen_expr_intro (Λ := spec_mod_lang (H := HSrcSpec) _ _ ) _ tt with "[Hγs_s] [-]"); [simpl; done..|]. *)
+(*     iEval (unfold echo_getc_spec). rewrite /TReceive bind_bind. *)
+(*     iApply (sim_src_TExist (H := HSrcSpec) (_, _, _)). *)
+(*     rewrite bind_bind. setoid_rewrite bind_ret_l. *)
+(*     iApply (sim_gen_TVis (H := HSrcSpec)). iIntros "% Hγs_s %% [-> [-> _ ]]". *)
+
+(*     iApply (sim_src_constP_next with "[Hγt] [Hγκ] [Hγs] [%] [-]"); [done..|]. *)
+(*     iDestruct (mstate_var_agree with "Hγs_s Hγs_s'") as "->". *)
+
+(*     iIntros "Hγs". iApply sim_gen_stop. *)
+(*     iApply (sim_tgt_constP_elim γt γs γκ with "[Hγs] [-]"); [done..|]. *)
+(*     iIntros "Hγs Hγt Hγκ". *)
+
+(*     iApply (sim_gen_expr_intro (Λ := spec_mod_lang (H := HSrcSpec) _ _ ) _ tt with "[Hγs_s] [-]"); [simpl; done..|]. *)
+(*     iApply (sim_src_TAssume (H := HSrcSpec)). iIntros (?). *)
+(*     iApply (sim_src_TAssume (H := HSrcSpec)). iIntros (?). simplify_eq. *)
+(*     iApply sim_gen_expr_None => /=. iIntros (? [] ?) "Hγs_s". *)
+
+(*     iIntros (??) "[-> [-> _]]". *)
+(*     rewrite bool_decide_true; [|done]. *)
+(*     iApply (sim_src_constP_next with "[Hγt] [Hγκ] [Hγs] [%] [-]"); [done..|]. *)
+(*     iIntros "Hγs". *)
+(*     iApply (sim_tgt_link_recv_left with "[-]"). *)
+(*     iApply (sim_tgt_rec_Waiting_raw _ []). *)
+(*     iSplit; [|by iIntros]. *)
+(*     iIntros (???? Hin) "!> %". simplify_map_eq. *)
+
+(*     (* Target's spec module (Right linking case - getc) *) *)
+(*     iMod (mstate_var_alloc (m_state (spec_trans rec_event Z))) as (γt_r) "Hγt_r". *)
+
+(*     iMod (mstate_var_alloc (list seq_product_case)) as (γt_q) "Hγt_q". *)
+
+(*     (* Linking event to pass around *) *)
+(*     iMod (mstate_var_alloc (option rec_ev)) as (γt_oe) "Hγt_oe". *)
+
+(*     iApply (sim_tgt_link_left_const_run γt_q γt_r γt_oe with "[$] [$] [$] [-]"). *)
+(*     iIntros "Hγt_q Hγt_r Hγt_oe". *)
+
+(*     iMod (rec_mapsto_alloc_big (h_heap h) with "Hh") as "[Hh _]". { apply map_disjoint_empty_r. } *)
+
+(*     iApply (sim_gen_expr_intro _ [] with "[Hh Ha]"). { done. } *)
+(*     { rewrite /= /rec_state_interp dom_empty_L right_id_L /=. iFrame "#∗". by iApply rec_alloc_fake. } *)
+
+(*     set (Π_s := sim_src_constP γκ γt (EV := rec_event) (m_t := m_t) (m_s := spec_trans rec_event Z)). *)
+(*     set (Π_t := tgt_link_left_constP _ _ _ _ _). *)
+
+(*     iApply (sim_gen_expr_bind _ [ReturnExtCtx _] with "[-]") => /=. *)
+
+(*     iDestruct (mstate_var_merge with "Hγs_s Hγs_s'") as "[% Hγs_s]". *)
+
+(*     rewrite /echo_prog in Hin. simplify_map_eq. *)
+
+
+
+(*     iApply (sim_echo_full with "[] [] [] Hγs Hγt_oe Hγt_q Hγt_r [//] [//]"). 1-3: by iApply (rec_fn_intro with "[$]") => /=. *)
+(*     { *)
+(*       iModIntro. iApply (sim_getc with "[//]"). by iApply (rec_fn_intro with "[$]"). *)
+(*       iIntros (??) => /=. *)
+(*       iDestruct 1 as (??) "[[Hγt_oe [Hγt_q Hγt_r]] [-> HC]]" => /=. *)
+
+(*       iIntros "%%% Hγt_q' Hγt_r' Hγt_oe'". *)
+
+(*       iDestruct (mstate_var_merge with "Hγt_r Hγt_r'") as "[<- Hγt_r]". *)
+(*       iDestruct (mstate_var_merge with "Hγt_oe Hγt_oe'") as "[<- Hγt_oe]". *)
+(*       iDestruct (mstate_var_merge with "Hγt_q Hγt_q'") as "[<- Hγt_q]". *)
+(*       iIntros (??????). destruct!/=. rewrite bool_decide_false //. rewrite bool_decide_true //. *)
+(*       iApply (sim_tgt_link_recv_right with "[-]"). iApply "HC". iSplit!. iIntros (??). iDestruct 1 as (? ->) "HC" => /=. *)
+(*       iIntros (?). simplify_eq. *)
+(*       iApply (sim_tgt_link_run_right with "[-]"). iApply "HC". iSplit!. *)
+(*       iIntros (??). iDestruct 1 as (??) "[% HC]" => /=. simplify_eq. *)
+(*       iIntros (??????). destruct!/=. *)
+(*       iApply (sim_tgt_link_left_const_recv γt_q γt_r γt_oe with "[$] [Hγt_r] [$] [-]"). 1: done. *)
+(*       iIntros "Hγt_q Hγt_r Hγt_oe". *)
+(*       iApply "HC". iSplit!. *)
+(*       iIntros (??). iDestruct 1 as (? ->) "HC" => /=. *)
+(*       iIntros "%%% Hγt_q' Hγt_r' Hγt_oe'". *)
+(*       iDestruct (mstate_var_merge with "Hγt_r Hγt_r'") as "[<- Hγt_r]". *)
+(*       iDestruct (mstate_var_merge with "Hγt_oe Hγt_oe'") as "[<- Hγt_oe]". *)
+(*       iDestruct (mstate_var_merge with "Hγt_q Hγt_q'") as "[<- Hγt_q]". iIntros (?). simplify_eq. *)
+(*       iApply (sim_tgt_link_left_const_run γt_q γt_r γt_oe with "[$] [Hγt_r] [$] [-]"). 1: done. *)
+(*       iIntros "Hγt_q Hγt_r Hγt_oe". *)
+(*       iApply ("HC" with "[-]"). iSplit!. iFrame. *)
+(*     } *)
+(*     { *)
+(*       (* iIntros "!> %% [% [% [% [[% [Hγs [% %]]] [[Hγt_oe [Hγt_q Hγt_r]] [-> HΦ]]]]]]". *) *)
+(*       iIntros "!> %% [% [% [% [HQ [HP [-> HΦ]]]]]]". *)
+(*       iApply (sim_echo_body _ _ (echo_left_external γs) (echo_left_linkP γt_oe γt_q γt_r) with "[] [] [-]"). 1 : by iApply (rec_fn_intro with "[$]"). *)
+(*       { *)
+(*         rewrite /switch_external_fixed => /=. *)
+(*         iIntros (??) "[% [% [% [% [% [% [[% [Hγs [% %]]] [[Hγt_oe [Hγt_q Hγt_r]] [% [% HC]]]]]]]]]]" => /=. *)
+(*         subst. iIntros (???) "Hγt_q' Hγt_r' Hγt_oe'". *)
+
+(*         iDestruct (mstate_var_merge with "Hγt_r Hγt_r'") as "[<- Hγt_r]". *)
+(*         iDestruct (mstate_var_merge with "Hγt_oe Hγt_oe'") as "[<- Hγt_oe]". *)
+(*         iDestruct (mstate_var_merge with "Hγt_q Hγt_q'") as "[<- Hγt_q]". *)
+(*         iIntros (??????). destruct!/=. rewrite bool_decide_false //. *)
+
+(*         iApply (sim_tgt_constP_elim γt γs γκ with "[Hγs] [-]"); [done..|]. *)
+(*         iIntros "Hγs Hγt Hγκ". *)
+(*         iApply "HC". iSplit!. *)
+
+(*         replace p with σ1.1 by admit. by destruct σ1. *)
+
+(*         iIntros (??). iDestruct 1 as (->) "HC". *)
+(*         iApply (sim_src_constP_next with "[Hγt] [Hγκ] [Hγs] [%] [-]"); [done..|]. *)
+(*         iIntros "Hγs". *)
+(*         iApply (sim_tgt_link_None with "[-]"). iIntros "!>" (??????). destruct!/=. *)
+(*         iApply (sim_tgt_constP_elim γt γs γκ with "[Hγs] [-]"); [done..|]. *)
+(*         iIntros "Hγs Hγt Hγκ". *)
+(*         iApply "HC". iSplit!. iIntros (??) "[% HC]". simplify_eq. *)
+(*         iApply (sim_src_constP_next with "[Hγt] [Hγκ] [Hγs] [%] [-]"); [done..|]. *)
+(*         iIntros "Hγs". iApply sim_gen_stop. *)
+(*         iApply (sim_tgt_constP_elim γt γs γκ with "[Hγs] [-]"); [done..|]. *)
+(*         iIntros "Hγs Hγt Hγκ". *)
+(*         iApply "HC". iSplit!. iIntros (??). iDestruct 1 as (?? -> ->) "[% [% HC]]". *)
+(*         iApply (sim_src_constP_next with "[Hγt] [Hγκ] [Hγs] [%] [-]"); [done..|]. *)
+(*         iIntros "Hγs". destruct!/=. *)
+(*         iApply (sim_tgt_link_left_const_recv γt_q γt_r γt_oe with "[$] [Hγt_r] [$] [-]"). 1: done. *)
+(*         iIntros "Hγt_q Hγt_r Hγt_oe". *)
+(*         iApply ("HC" with "[-]"). iFrame. iSplit!. *)
+(*         iIntros (??). iDestruct 1 as (? ->) "HC". *)
+(*         iIntros (???) "Hγt_q' Hγt_r' Hγt_oe'". *)
+
+(*         iDestruct (mstate_var_merge with "Hγt_r Hγt_r'") as "[<- Hγt_r]". *)
+(*         iDestruct (mstate_var_merge with "Hγt_oe Hγt_oe'") as "[<- Hγt_oe]". *)
+(*         iDestruct (mstate_var_merge with "Hγt_q Hγt_q'") as "[<- Hγt_q]". *)
+(*         iIntros (?). simplify_eq. *)
+
+(*         iApply (sim_tgt_link_left_const_run γt_q γt_r γt_oe with "[$] [Hγt_r] [$] [-]"). 1: done. *)
+(*         iIntros "???". *)
+
+(*         iApply "HC". iSplit!. *)
+(*         iFrame. iSplit!. *)
+(*       } *)
+(*       unfold putc_echo_fn_spec => /=. *)
+(*       iSplit!. by iFrame. *)
+(*     } *)
+(*     iSplit!. *)
+(*     iIntros (?) "[% [% [% [Hγs [% [Hγt_oe [Hγt_q Hγt_r]]]]]]]". *)
+(*     iApply sim_tgt_rec_ReturnExt. iIntros (???) "#? ? ? !> %% [% [% ?]] /=". *)
+(*     subst. *)
+(*     iIntros (???) "???". *)
+
+(*     iDestruct (mstate_var_merge with "Hγt_r [$]") as "[<- Hγt_r]". *)
+(*     iDestruct (mstate_var_merge with "Hγt_oe [$]") as "[<- Hγt_oe]". *)
+(*     iDestruct (mstate_var_merge with "Hγt_q [$]") as "[<- Hγt_q]". *)
+(*     iIntros (??????). destruct!/=. *)
+
+(*     iApply (sim_tgt_constP_elim γt γs γκ with "[Hγs] [-]"); [done..|]. *)
+(*     iIntros "Hγs Hγt Hγκ". *)
+
+(*     iMod (mstate_var_split γs_s σs.2 with "[$]") as "[Hγs_s Hγs_s']". *)
+(*     iApply (sim_gen_expr_intro _ tt with "[Hγs_s]"); simpl; [done..|]. *)
+(*     iApply (sim_src_TExist with "[-]"). *)
+(*     iApply (sim_gen_TVis with "[-]"). *)
+(*     iIntros (?) "Hγs_s %% [% [% ?]] /=". *)
+
+(*     iApply (sim_src_constP_elim with "[Hγt] [Hγκ] [-]"); [done..|]. *)
+(*     iIntros "Hγt Hγκ". iSplit!. *)
+
+(*     iApply (sim_tgt_constP_intro γt γs γκ with "[Hγt] [Hγs] [Hγκ] [-]"); [done..|]. *)
+(*     iIntros "Hγs". *)
+
+(*     iApply (sim_tgt_link_None with "[-]"). iIntros "!>" (??????). *)
+(*     destruct!/=. case_match; destruct!/=. *)
+
+(*     iApply (sim_tgt_constP_elim γt γs γκ with "[Hγs] [-]"); [done..|]. *)
+(*     iIntros "Hγs Hγt Hγκ". *)
+(*     iApply (sim_gen_expr_intro _ tt with "[Hγs_s]"); simpl; [done..|]. *)
+(*     iApply sim_src_TUb_end. *)
+(*     Admitted. *)
+
+(* End echo_getc. *)
